Engine: new suggestion of PikeVM prefix invariant
I hope that this definition, prefix_inv, can replace nextt_nextprefix entirely.
With this version, one could probably remove pike_tree_nextt_shape entirely.
To show that this is still strong enough to imply this shape, I've added lemmas
showing that trees related by this invariant are trees of some actions involving
the dot_star.

Engine/PikeEquiv.v
@@ -485,7 +485,7 @@ Qed.
 
 
 
-(** * Simulation Invariant  *)
+(** * Simulation Invariant: inclusion of seen sets  *)
 
 (* This is not, strictly speaking, an inclusion, which explains the second case of this disjunction *)
 (* Sometimes, we add seen pcs on the VM side that do not correspond yet to any seen tree on the tree side *)
@@ -509,6 +509,8 @@ Definition head_pc (threadactive:list thread) : label :=
   | (pc,_,_)::_ => pc
   end.
 
+(** * Simulation Invariant: old version of relating next tree and next prefix  *)
+
 (* Simulation invariant between the nextt tree and the nextprefix *)
 Inductive nextt_nextprefix (code:code): input -> option tree -> option (nat * literal) -> Prop :=
 | nnp_none: forall inp, nextt_nextprefix code inp None None
@@ -524,13 +526,171 @@ Inductive nextt_nextprefix (code:code): input -> option tree -> option (nat * li
     nextt_nextprefix code (Input (c::next) pref) (Some nextt) (Some (S n, lit))
 | nnp_generate:
   forall c next pref nextt t1 t2 r lit
-    (NEXTT: nextt = Some (lazy_tree c t1 t2))
+    (NEXTT: nextt = lazy_tree c t1 t2)
     (COMPILE: compilation r = code)
     (SUBSET: pike_regex r)
     (T1: bool_tree rer [Areg r] (Input next (c::pref)) CanExit t1)
     (T2: pike_tree_nextt_shape rer r (Input next (c::pref)) t2)
     (LIT: extract_literal r = lit),
-    nextt_nextprefix code (Input (c::next) pref) nextt (Some (0, lit)).
+    nextt_nextprefix code (Input (c::next) pref) (Some nextt) (Some (0, lit)).
+
+
+(** * Simulation Invariant: Invariant of unanchored next tree and next prefix  *)
+
+(* How to relate the `nextt` prefix of PikeTree to the `next_prefix` of PikeVM?
+
+  Whenever `next_prefix` is None, it means that string search did not find a
+  match for the prefix in the remainder of the string.
+  We can find a PikeTre behavior where `nextt` is also None, because the
+  remaining unanchored tree `nextt` cannot contain any matching leaf.
+
+  In particular, when the input is at the end (`Input [] pref`), then
+  `next_prefix` has to be None, and we will also have `nextt = None`.
+
+  When `next_prefix` is `Some (n, lit)`, we know that at the next `n` positions,
+  there cannot be a match.
+  In the unanchored tree `nextt` corresponding to the remaining positions,
+  we know that the `n` first left subtrees will have no results.
+
+  In any case, the `nextt` is equal to Some tree, since we may still find
+  unanchored results at later positions.
+  This unanchored tree has a particular shape: since it describes what will
+  happen at the next positions (not including the current one),
+  it starts with a `Read` to advance, a progress check,
+  then a choice between trying to find a match of the regex at the next
+  input position, or resetting no group and then recursively describing
+  what happens for the next positions.
+  Only when `n>0` do we know for sure that the tree of the next input position
+  has no result.
+ *)
+
+
+(* `next_prefix_tree r inp n t` means that:
+   - t is the unanchored tree that corresponds to trying to match `r` from the next position
+   - the `n` next input positions do not contain a match for `r`
+   This tree `t` is either a `Mismatch` when there is no such next position.
+   Or it has a distinct shape, starting with a `Read` to go to the next input position,
+   then a choice between trying to match `r` and iterating.
+ *)
+Inductive next_prefix_tree (r:regex): input -> nat -> tree -> Prop :=
+| np_end:
+  forall pref n,
+    next_prefix_tree r (Input [] pref) n Mismatch
+| np_0:
+  forall next pref c t1 t2 nextt n
+    (NEXTT: nextt = lazy_tree c t1 t2)
+    (ISTREE: bool_tree rer [Areg r] (Input next (c::pref)) CanExit t1)
+    (NEXT: next_prefix_tree r (Input next (c::pref)) n t2),
+    next_prefix_tree r (Input (c::next) pref) 0 nextt
+| np_S:
+  forall next pref c t1 t2 nextt n
+    (NEXTT: nextt = lazy_tree c t1 t2)
+    (ISTREE: bool_tree rer [Areg r] (Input next (c::pref)) CanExit t1)
+    (NORES: first_leaf t1 (Input next (c::pref)) = None)
+    (NEXT: next_prefix_tree r (Input next (c::pref)) n t2),
+    next_prefix_tree r (Input (c::next) pref) (S n) nextt.
+
+Inductive prefix_inv (code:code): input -> option tree -> option (nat*literal) -> Prop :=
+| pi_none: forall inp, prefix_inv code inp None None
+(* The Some case can only happen when the input is not at the end *)
+| pi_some:
+  forall r next pref c nextt n lit
+    (COMPILE: compilation r = code)
+    (SUBSET: pike_regex r)
+    (LIT: extract_literal r = lit)
+    (PREFINV: next_prefix_tree r (Input (c::next) pref) n nextt),
+    prefix_inv code (Input (c::next) pref) (Some nextt) (Some (n, lit)).
+
+(* when the invariant hold, we know that the tree has the shape of an
+   unanchored tree of [.*?r] *)
+Lemma shape_next_prefix_tree_0:
+  forall r inp nextt,
+    next_prefix_tree r inp 0 nextt <->
+    bool_tree rer [Areg (Regex.Character CdAll); Acheck inp; Areg (Quantified false 0 +∞ (Regex.Character CdAll)); Areg r] inp CannotExit nextt.
+Proof.
+  intros r inp nextt.
+  split.
+  - generalize 0 at 1. intros n NEXT. induction NEXT.
+    + constructor. simpl. auto.
+    + subst. econstructor; simpl; eauto. (* read *)
+      econstructor.                      (* progress *)
+      replace +∞ with (NoI.N 1 + +∞)%NoI by (simpl; auto).
+      econstructor; simpl; eauto.        (* choice *)
+    + subst. econstructor; simpl; eauto. (* read *)
+      econstructor.                      (* progress *)
+      replace +∞ with (NoI.N 1 + +∞)%NoI by (simpl; auto).
+      econstructor; eauto.        (* choice *)
+  - intros TREE. destruct inp as [next pref].
+    generalize dependent pref. generalize dependent nextt.
+    induction next; intros.
+    { inversion TREE; subst; inversion READ. constructor. }
+    inversion TREE; subst.      (* read *)
+    2: { inversion READ. }
+    inversion TREECONT; subst.  (* progress *)
+    inversion TREECONT0; subst. (* choice *)
+    destruct plus; inversion H1.
+    simpl in READ. inversion READ. subst.
+    eapply np_0; simpl; eauto.
+Qed.
+
+(* reducing the number of empty subtrees weakens the property *)
+Lemma next_prefix_tree_weaken:
+  forall r inp nextt n1 n2,
+    n2 < n1 ->
+    next_prefix_tree r inp n1 nextt ->
+    next_prefix_tree r inp n2 nextt.
+Proof.
+  intros r inp nextt n1 n2 LT NEXT.
+  generalize dependent n2.
+  induction NEXT; intros; [constructor|lia|].
+  destruct n2 as [|n2].
+  - econstructor; eauto.
+  - econstructor; eauto.
+    apply IHNEXT. lia.
+Qed.
+
+Corollary shape_next_prefix_tree:
+  forall r inp nextt n,
+    next_prefix_tree r inp n nextt ->
+    bool_tree rer [Areg (Regex.Character CdAll); Acheck inp; Areg (Quantified false 0 +∞ (Regex.Character CdAll)); Areg r] inp CannotExit nextt.
+Proof.
+  intros r inp nextt n H.
+  apply shape_next_prefix_tree_0.
+  destruct n; auto.
+  apply next_prefix_tree_weaken with (n2:=0) in H; [auto|lia].
+Qed.
+
+Lemma shape_prefix_tree:
+  forall r n inp nextt tnow,
+    next_prefix_tree r inp n nextt ->
+    bool_tree rer [Areg r] inp CanExit tnow ->
+    bool_tree rer [Areg dot_star; Areg r] inp CanExit (Choice tnow (GroupAction (Reset []) nextt)).
+Proof.
+  intros r n inp nextt tnow NEXT NOW.
+  unfold dot_star. replace +∞ with (NoI.N 1 + +∞)%NoI by (simpl; auto).
+  econstructor; simpl; eauto.
+  eapply shape_next_prefix_tree; eauto.
+Qed.
+  
+(* an alternative version that only talks about the next position *)
+Lemma prefix_tree_shape:
+  forall r n next pref c t1 t2,
+    pike_regex r ->
+    next_prefix_tree r (Input (c::next) pref) n (lazy_tree c t1 t2) ->
+    bool_tree rer ([Areg dot_star; Areg r]) (Input next (c::pref)) CanExit (Choice t1 (GroupAction (Reset []) t2)).
+Proof.
+  intros r n next pref c t1 t2 SUBSET NEXT.
+  specialize (FunctionalUtils.is_tree_productivity rer [Areg r] (Input (c::next) pref) GroupMap.empty forward) as [tnow TREE].
+  eapply shape_prefix_tree in NEXT; eauto.
+  - inversion NEXT. destruct plus; inversion H1. subst.
+    simpl in CHOICE. inversion CHOICE; subst.
+    inversion ISTREE1; subst.
+    inversion TREECONT; subst.
+    simpl in READ. inversion READ. subst. eauto.
+  - eapply encode_equal; repeat constructor; eauto.
+Qed.
+
+(** * Simulation Invariant  *)
 
 Inductive pike_inv (code:code): pike_tree_state -> pike_vm_state -> Prop :=
 | pikeinv:
@@ -752,8 +912,7 @@ Proof.
     eauto using acc_skip.
 
     simpl; now rewrite <-app_assoc.
-  - injection NEXTT as ->.
-    simpl. eauto using acc_keep.
+  - simpl. eauto using acc_keep.
 Qed.
 
 Lemma initial_nextt_nextprefix {strs:StrSearch}:
@@ -1082,7 +1241,6 @@ Proof.
           inversion NEXTTPREFIX; subst.
           - eauto 10 using pike_tree_acc_bool_tree.
           - assert (t1 = t /\ t2 = acc) as [? ?]. {
-              injection NEXTT as ->.
               inversion TREEACC; subst.
               - now injection NEXTT.
               - injection INPUT as <-; subst.
